Update SimMemory.v

src/opt/SimMemory.v
@@ -24,6 +24,23 @@ Require Import Configuration.
 Set Implicit Arguments.
 
 
+Inductive sim_message: forall (msg_src msg_tgt: Message.t), Prop :=
+| sim_message_full
+    val released_src released_tgt
+    (RELEASED: View.opt_le released_src released_tgt):
+    sim_message (Message.mk val released_src) (Message.mk val released_tgt)
+| sim_message_half:
+    sim_message Message.half Message.half
+.
+
+Program Instance sim_message_PreOrder: PreOrder sim_message.
+Next Obligation.
+  ii. destruct x; econs; refl.
+Qed.
+Next Obligation.
+  ii. inv H; inv H0; econs. etrans; eauto.
+Qed.
+
 Inductive covered (loc:Loc.t) (ts:Time.t) (mem:Memory.t): Prop :=
 | covered_intro
     from to msg
@@ -34,11 +51,11 @@ Inductive covered (loc:Loc.t) (ts:Time.t) (mem:Memory.t): Prop :=
 Inductive sim_memory (mem_src mem_tgt:Memory.t): Prop :=
 | sim_memory_intro
     (COVER: forall loc ts, covered loc ts mem_src <-> covered loc ts mem_tgt)
-    (MSG: forall loc from_tgt to val released_tgt
-            (GET: Memory.get loc to mem_tgt = Some (from_tgt, Message.mk val released_tgt)),
-        exists from_src released_src,
-          <<GET: Memory.get loc to mem_src = Some (from_src, Message.mk val released_src)>> /\
-          <<RELEASED: View.opt_le released_src released_tgt>>)
+    (MSG: forall loc from_tgt to msg_tgt
+            (GET: Memory.get loc to mem_tgt = Some (from_tgt, msg_tgt)),
+        exists from_src msg_src,
+          <<GET: Memory.get loc to mem_src = Some (from_src, msg_src)>> /\
+          <<MSG: sim_message msg_src msg_tgt>>)
 .
 
 Program Instance sim_memory_PreOrder: PreOrder sim_memory.
@@ -49,66 +66,69 @@ Next Obligation.
   ii. inv H. inv H0. econs; try etrans; eauto. i.
   exploit MSG0; eauto. i. des.
   exploit MSG; eauto. i. des.
-  esplits; eauto.
+  esplits; eauto. etrans; eauto.
 Qed.
 
 
 Lemma sim_memory_get
-      loc from_tgt to val released_tgt mem_src mem_tgt
+      loc from_tgt to msg_tgt mem_src mem_tgt
       (SIM: sim_memory mem_src mem_tgt)
-      (GET: Memory.get loc to mem_tgt = Some (from_tgt, Message.mk val released_tgt)):
-  exists from_src released_src,
-    <<GET: Memory.get loc to mem_src = Some (from_src, Message.mk val released_src)>> /\
-    <<RELEASED: View.opt_le released_src released_tgt>>.
+      (GET: Memory.get loc to mem_tgt = Some (from_tgt, msg_tgt)):
+  exists from_src msg_src,
+    <<GET: Memory.get loc to mem_src = Some (from_src, msg_src)>> /\
+    <<MSG: sim_message msg_src msg_tgt>>.
 Proof.
   eapply SIM. eauto.
 Qed.
 
-Lemma sim_memory_max_timemap
-      mem_src mem_tgt
-      (CLOSED_SRC: Memory.closed mem_src)
-      (CLOSED_TGT: Memory.closed mem_tgt)
-      (SIM: sim_memory mem_src mem_tgt):
-  TimeMap.le (Memory.max_timemap mem_src) (Memory.max_timemap mem_tgt).
-Proof.
-  apply Memory.max_timemap_spec'; try by apply CLOSED_TGT; auto. i.
-  destruct (Time.le_lt_dec (Memory.max_timemap mem_src loc) Time.bot).
-  { esplits; eauto. apply CLOSED_TGT. }
-  exploit Memory.max_timemap_closed; try apply CLOSED_SRC; eauto.
-  instantiate (1 := loc). i. des.
-  inv SIM. destruct (COVER loc (Memory.max_timemap mem_src loc)) as [C1 C2].
-  exploit C1; eauto.
-  { econs; eauto. apply Interval.mem_ub.
-    destruct (mem_src loc).(Cell.WF). exploit VOLUME; eauto. i. des; auto.
-    inv x. rewrite H1 in *. inv l.
-  }
-  i. inv x. inv ITV. destruct msg. ss.
-  esplits; eauto.
-Qed.
+(* Lemma sim_memory_max_timemap *)
+(*       mem_src mem_tgt mtm_src mtm_tgt *)
+(*       (CLOSED_SRC: Memory.closed mem_src) *)
+(*       (CLOSED_TGT: Memory.closed mem_tgt) *)
+(*       (SIM: sim_memory mem_src mem_tgt) *)
+(*       (MAX_SRC: Memory.max_full_timemap mem_src mtm_src) *)
+(*       (MAX_TGT: Memory.max_full_timemap mem_tgt mtm_tgt): *)
+(*   mtm_src = mtm_tgt. *)
+(* Proof. *)
+(*   apply TimeMap.antisym. *)
+(*   - eapply Memory.max_full_timemap_spec'; eauto. i. *)
+(*     destruct (Time.le_lt_dec (mtm_src loc) Time.bot). *)
+(*     { esplits; eauto. apply CLOSED_TGT. } *)
+(*     exploit Memory.max_full_timemap_closed; try apply MAX_SRC; eauto. *)
+(*     instantiate (1 := loc). i. des. *)
+(*     inv SIM. destruct (COVER loc (mtm_src loc)) as [C1 C2]. *)
+(*     exploit C1; eauto. *)
+(*     { econs; eauto. apply Interval.mem_ub. *)
+(*       destruct (mem_src loc).(Cell.WF). exploit VOLUME; eauto. i. des; auto. *)
+(*       inv x. rewrite H1 in *. inv l. *)
+(*     } *)
+(*     i. inv x. inv ITV. destruct msg. ss. *)
+(*     esplits; eauto. *)
+(* Qed. *)
 
-Lemma sim_memory_max_view
-      mem_src mem_tgt
-      (CLOSED_SRC: Memory.closed mem_src)
-      (CLOSED_TGT: Memory.closed mem_tgt)
-      (SIM: sim_memory mem_src mem_tgt):
-  View.le (Memory.max_view mem_src) (Memory.max_view mem_tgt).
-Proof.
-  econs; apply sim_memory_max_timemap; auto.
-Qed.
+(* Lemma sim_memory_max_view *)
+(*       mem_src mem_tgt *)
+(*       (CLOSED_SRC: Memory.closed mem_src) *)
+(*       (CLOSED_TGT: Memory.closed mem_tgt) *)
+(*       (SIM: sim_memory mem_src mem_tgt): *)
+(*   View.le (Memory.max_view mem_src) (Memory.max_view mem_tgt). *)
+(* Proof. *)
+(*   econs; apply sim_memory_max_timemap; auto. *)
+(* Qed. *)
 
-Lemma sim_memory_max_released
-      mem_src mem_tgt loc ts
-      (CLOSED_SRC: Memory.closed mem_src)
-      (CLOSED_TGT: Memory.closed mem_tgt)
-      (SIM: sim_memory mem_src mem_tgt):
-  View.le (Memory.max_released mem_src loc ts) (Memory.max_released mem_tgt loc ts).
-Proof.
-  unfold Memory.max_released. econs; s.
-  - ii. unfold TimeMap.add. condtac; [refl|].
-    eapply sim_memory_max_timemap; eauto.
-  - ii. unfold TimeMap.add. condtac; [refl|].
-    eapply sim_memory_max_timemap; eauto.
-Qed.
+(* Lemma sim_memory_max_released *)
+(*       mem_src mem_tgt loc ts *)
+(*       (CLOSED_SRC: Memory.closed mem_src) *)
+(*       (CLOSED_TGT: Memory.closed mem_tgt) *)
+(*       (SIM: sim_memory mem_src mem_tgt): *)
+(*   View.le (Memory.max_released mem_src loc ts) (Memory.max_released mem_tgt loc ts). *)
+(* Proof. *)
+(*   unfold Memory.max_released. econs; s. *)
+(*   - ii. unfold TimeMap.add. condtac; [refl|]. *)
+(*     eapply sim_memory_max_timemap; eauto. *)
+(*   - ii. unfold TimeMap.add. condtac; [refl|]. *)
+(*     eapply sim_memory_max_timemap; eauto. *)
+(* Qed. *)
 
 Lemma covered_disjoint
       mem1 mem2 loc from to
@@ -142,9 +162,9 @@ Proof.
 Qed.
 
 Lemma add_covered
-      mem2 mem1 loc from to val released
+      mem2 mem1 loc from to msg
       l t
-      (ADD: Memory.add mem1 loc from to val released mem2):
+      (ADD: Memory.add mem1 loc from to msg mem2):
   covered l t mem2 <->
   covered l t mem1 \/ (l = loc /\ Interval.mem (from, to) t).
 Proof.
@@ -161,9 +181,9 @@ Proof.
 Qed.
 
 Lemma split_covered
-      mem2 mem1 loc ts1 ts2 ts3 val2 val3 released2 released3
+      mem2 mem1 loc ts1 ts2 ts3 msg2 msg3
       l t
-      (SPLIT: Memory.split mem1 loc ts1 ts2 ts3 val2 val3 released2 released3 mem2):
+      (SPLIT: Memory.split mem1 loc ts1 ts2 ts3 msg2 msg3 mem2):
   covered l t mem2 <-> covered l t mem1.
 Proof.
   econs; i.
@@ -203,9 +223,9 @@ Proof.
 Qed.
 
 Lemma lower_covered
-      mem2 mem1 loc from to val released1 released2
+      mem2 mem1 loc from to msg1 msg2
       l t
-      (LOWER: Memory.lower mem1 loc from to val released1 released2 mem2):
+      (LOWER: Memory.lower mem1 loc from to msg1 msg2 mem2):
   covered l t mem2 <-> covered l t mem1.
 Proof.
   econs; i.
@@ -225,12 +245,12 @@ Proof.
 Qed.
 
 Lemma sim_memory_add
-      mem1_src mem1_tgt released_src
-      mem2_src mem2_tgt released_tgt
-      loc from to val
-      (REL_LE: View.opt_le released_src released_tgt)
-      (SRC: Memory.add mem1_src loc from to val released_src mem2_src)
-      (TGT: Memory.add mem1_tgt loc from to val released_tgt mem2_tgt)
+      mem1_src mem1_tgt msg_src
+      mem2_src mem2_tgt msg_tgt
+      loc from to
+      (SIM_MSG: sim_message msg_src msg_tgt)
+      (SRC: Memory.add mem1_src loc from to msg_src mem2_src)
+      (TGT: Memory.add mem1_tgt loc from to msg_tgt mem2_tgt)
       (SIM: sim_memory mem1_src mem1_tgt):
   sim_memory mem2_src mem2_tgt.
 Proof.
@@ -248,10 +268,10 @@ Qed.
 Lemma sim_memory_split
       mem1_src mem1_tgt
       mem2_src mem2_tgt
-      loc ts1 ts2 ts3 val2 val3 released2_src released3_src released2_tgt released3_tgt
-      (REL_LE: View.opt_le released2_src released2_tgt)
-      (SRC: Memory.split mem1_src loc ts1 ts2 ts3 val2 val3 released2_src released3_src mem2_src)
-      (TGT: Memory.split mem1_tgt loc ts1 ts2 ts3 val2 val3 released2_tgt released3_tgt mem2_tgt)
+      loc ts1 ts2 ts3 msg2_src msg3_src msg2_tgt msg3_tgt
+      (SIM_MSG: sim_message msg2_src msg2_tgt)
+      (SRC: Memory.split mem1_src loc ts1 ts2 ts3 msg2_src msg3_src mem2_src)
+      (TGT: Memory.split mem1_tgt loc ts1 ts2 ts3 msg2_tgt msg3_tgt mem2_tgt)
       (SIM: sim_memory mem1_src mem1_tgt):
   sim_memory mem2_src mem2_tgt.
 Proof.
@@ -273,10 +293,10 @@ Qed.
 Lemma sim_memory_lower
       mem1_src mem1_tgt
       mem2_src mem2_tgt
-      loc from to val released1_src released1_tgt released2_src released2_tgt
-      (REL_LE: View.opt_le released2_src released2_tgt)
-      (SRC: Memory.lower mem1_src loc from to val released1_src released2_src mem2_src)
-      (TGT: Memory.lower mem1_tgt loc from to val released1_tgt released2_tgt mem2_tgt)
+      loc from to msg1_src msg2_src msg1_tgt msg2_tgt
+      (SIM_MSG: sim_message msg2_src msg2_tgt)
+      (SRC: Memory.lower mem1_src loc from to msg1_src msg2_src mem2_src)
+      (TGT: Memory.lower mem1_tgt loc from to msg1_tgt msg2_tgt mem2_tgt)
       (SIM: sim_memory mem1_src mem1_tgt):
   sim_memory mem2_src mem2_tgt.
 Proof.
@@ -290,12 +310,12 @@ Proof.
 Qed.
 
 Lemma sim_memory_promise
-      loc from to val kind
-      promises1_src mem1_src released_src promises2_src mem2_src
-      promises1_tgt mem1_tgt released_tgt promises2_tgt mem2_tgt
-      (REL_LE: View.opt_le released_src released_tgt)
-      (PROMISE_SRC: Memory.promise promises1_src mem1_src loc from to val released_src promises2_src mem2_src kind)
-      (PROMISE_TGT: Memory.promise promises1_tgt mem1_tgt loc from to val released_tgt promises2_tgt mem2_tgt kind)
+      loc from to kind
+      promises1_src mem1_src msg_src promises2_src mem2_src
+      promises1_tgt mem1_tgt msg_tgt promises2_tgt mem2_tgt
+      (SIM_MSG: sim_message msg_src msg_tgt)
+      (PROMISE_SRC: Memory.promise promises1_src mem1_src loc from to msg_src promises2_src mem2_src kind)
+      (PROMISE_TGT: Memory.promise promises1_tgt mem1_tgt loc from to msg_tgt promises2_tgt mem2_tgt kind)
       (SIM: sim_memory mem1_src mem1_tgt):
   sim_memory mem2_src mem2_tgt.
 Proof.
@@ -313,7 +333,8 @@ Lemma sim_memory_closed_timemap
   Memory.closed_timemap tm mem_src.
 Proof.
   ii. exploit TGT; eauto. i. des.
-  exploit sim_memory_get; eauto. i. des. eauto.
+  exploit sim_memory_get; eauto. i. des.
+  inv MSG. eauto.
 Qed.
 
 Lemma sim_memory_closed_view
@@ -339,8 +360,8 @@ Proof.
 Qed.
 
 Lemma lower_sim_memory
-      mem1 loc from to val released1 released2 mem2
-      (LOWER: Memory.lower mem1 loc from to val released1 released2 mem2):
+      mem1 loc from to val released1 msg2 mem2
+      (LOWER: Memory.lower mem1 loc from to (Message.mk val released1) msg2 mem2):
   sim_memory mem2 mem1.
 Proof.
   econs.
@@ -348,22 +369,22 @@ Proof.
   - i. erewrite Memory.lower_o; eauto. condtac; ss.
     + des. subst.
       exploit Memory.lower_get0; eauto. i. des.
-      rewrite GET0 in GET. inv GET.
-      esplits; eauto.
+      rewrite GET0 in GET. inv GET. inv MSG_LE.
+      esplits; eauto. econs; eauto.
     + esplits; eauto. refl.
 Qed.
 
 Lemma promise_lower_sim_memory
-      promises1 mem1 loc from to val released1 released2 promises2 mem2
-      (PROMISE: Memory.promise promises1 mem1 loc from to val released2 promises2 mem2 (Memory.op_kind_lower released1)):
+      promises1 mem1 loc from to val released1 msg2 promises2 mem2
+      (PROMISE: Memory.promise promises1 mem1 loc from to msg2 promises2 mem2 (Memory.op_kind_lower (Message.mk val released1))):
   sim_memory mem2 mem1.
 Proof.
   inv PROMISE. eapply lower_sim_memory. eauto.
 Qed.
 
 Lemma split_sim_memory
-      mem0 loc ts1 ts2 ts3 val2 val3 released2 released3 mem1
-      (SPLIT: Memory.split mem0 loc ts1 ts2 ts3 val2 val3 released2 released3 mem1):
+      mem0 loc ts1 ts2 ts3 msg2 msg3 mem1
+      (SPLIT: Memory.split mem0 loc ts1 ts2 ts3 msg2 msg3 mem1):
   sim_memory mem1 mem0.
 Proof.
   econs.
